---


---

<h1 id="cs341-agenda-tomorrow">CS341 Agenda (Tomorrow)</h1>
<h2 id="using-change-of-variable-example">Using change of variable, example:</h2>
<p>Sometimes, a little algebraic manipulation can make an unknown recurrence similar<br>
to one you have seen before. As an example, consider the recurrence<br>
<span class="katex--display"><span class="katex-display"><span class="katex"><span class="katex-mathml"><math><semantics><mrow><mi>T</mi><mo stretchy="false">(</mo><mi>n</mi><mo stretchy="false">)</mo><mo>=</mo><mn>2</mn><mi>T</mi><mo stretchy="false">(</mo><mo stretchy="false">⌈</mo><mi>n</mi><mo stretchy="false">⌉</mo><mo stretchy="false">)</mo><mo>+</mo><mi>l</mi><mi>g</mi><mo stretchy="false">(</mo><mi>n</mi><mo stretchy="false">)</mo></mrow><annotation encoding="application/x-tex">
T(n) = 2T(\lceil n\rceil)+lg(n)
</annotation></semantics></math></span><span class="katex-html" aria-hidden="true"><span class="base"><span class="strut" style="height: 1em; vertical-align: -0.25em;"></span><span class="mord mathdefault" style="margin-right: 0.13889em;">T</span><span class="mopen">(</span><span class="mord mathdefault">n</span><span class="mclose">)</span><span class="mspace" style="margin-right: 0.277778em;"></span><span class="mrel">=</span><span class="mspace" style="margin-right: 0.277778em;"></span></span><span class="base"><span class="strut" style="height: 1em; vertical-align: -0.25em;"></span><span class="mord">2</span><span class="mord mathdefault" style="margin-right: 0.13889em;">T</span><span class="mopen">(</span><span class="mopen">⌈</span><span class="mord mathdefault">n</span><span class="mclose">⌉</span><span class="mclose">)</span><span class="mspace" style="margin-right: 0.222222em;"></span><span class="mbin">+</span><span class="mspace" style="margin-right: 0.222222em;"></span></span><span class="base"><span class="strut" style="height: 1em; vertical-align: -0.25em;"></span><span class="mord mathdefault" style="margin-right: 0.01968em;">l</span><span class="mord mathdefault" style="margin-right: 0.03588em;">g</span><span class="mopen">(</span><span class="mord mathdefault">n</span><span class="mclose">)</span></span></span></span></span></span><br>
which looks difficult. We can simplify this recurrence, though, with a change of variables.<br>
For convenience, we shall not worry about rounding off values, such as <span class="katex--inline"><span class="katex"><span class="katex-mathml"><math><semantics><mrow><msqrt><mo stretchy="false">(</mo></msqrt><mi>n</mi><mo stretchy="false">)</mo></mrow><annotation encoding="application/x-tex">\sqrt(n)</annotation></semantics></math></span><span class="katex-html" aria-hidden="true"><span class="base"><span class="strut" style="height: 1.24em; vertical-align: -0.305em;"></span><span class="mord sqrt"><span class="vlist-t vlist-t2"><span class="vlist-r"><span class="vlist" style="height: 0.935em;"><span class="svg-align" style="top: -3.2em;"><span class="pstrut" style="height: 3.2em;"></span><span class="mopen" style="padding-left: 1em;">(</span></span><span class="" style="top: -2.895em;"><span class="pstrut" style="height: 3.2em;"></span><span class="hide-tail" style="min-width: 1.02em; height: 1.28em;"><svg width="400em" height="1.28em" viewBox="0 0 400000 1296" preserveAspectRatio="xMinYMin slice"><path d="M263,681c0.7,0,18,39.7,52,119c34,79.3,68.167,
158.7,102.5,238c34.3,79.3,51.8,119.3,52.5,120c340,-704.7,510.7,-1060.3,512,-1067
c4.7,-7.3,11,-11,19,-11H40000v40H1012.3s-271.3,567,-271.3,567c-38.7,80.7,-84,
175,-136,283c-52,108,-89.167,185.3,-111.5,232c-22.3,46.7,-33.8,70.3,-34.5,71
c-4.7,4.7,-12.3,7,-23,7s-12,-1,-12,-1s-109,-253,-109,-253c-72.7,-168,-109.3,
-252,-110,-252c-10.7,8,-22,16.7,-34,26c-22,17.3,-33.3,26,-34,26s-26,-26,-26,-26
s76,-59,76,-59s76,-60,76,-60z M1001 80H40000v40H1012z"></path></svg></span></span></span><span class="vlist-s">​</span></span><span class="vlist-r"><span class="vlist" style="height: 0.305em;"><span class=""></span></span></span></span></span><span class="mord mathdefault">n</span><span class="mclose">)</span></span></span></span></span><br>
to be integers. Renaming <span class="katex--inline"><span class="katex"><span class="katex-mathml"><math><semantics><mrow><mi>m</mi><mo>=</mo><mi>l</mi><mi>g</mi><mo stretchy="false">(</mo><mi>n</mi><mo stretchy="false">)</mo></mrow><annotation encoding="application/x-tex">m = lg(n)</annotation></semantics></math></span><span class="katex-html" aria-hidden="true"><span class="base"><span class="strut" style="height: 0.43056em; vertical-align: 0em;"></span><span class="mord mathdefault">m</span><span class="mspace" style="margin-right: 0.277778em;"></span><span class="mrel">=</span><span class="mspace" style="margin-right: 0.277778em;"></span></span><span class="base"><span class="strut" style="height: 1em; vertical-align: -0.25em;"></span><span class="mord mathdefault" style="margin-right: 0.01968em;">l</span><span class="mord mathdefault" style="margin-right: 0.03588em;">g</span><span class="mopen">(</span><span class="mord mathdefault">n</span><span class="mclose">)</span></span></span></span></span> yields:<br>
<span class="katex--display"><span class="katex-display"><span class="katex"><span class="katex-mathml"><math><semantics><mrow><mi>T</mi><mo stretchy="false">(</mo><msup><mn>2</mn><mi>m</mi></msup><mo stretchy="false">)</mo><mo>=</mo><mn>2</mn><mi>T</mi><mo stretchy="false">(</mo><msup><mn>2</mn><mrow><mn>2</mn><mi mathvariant="normal">/</mi><mi>m</mi></mrow></msup><mo stretchy="false">)</mo><mo>+</mo><mi>m</mi></mrow><annotation encoding="application/x-tex">
T(2^m) = 2T (2^{2/m})+ m 
</annotation></semantics></math></span><span class="katex-html" aria-hidden="true"><span class="base"><span class="strut" style="height: 1em; vertical-align: -0.25em;"></span><span class="mord mathdefault" style="margin-right: 0.13889em;">T</span><span class="mopen">(</span><span class="mord"><span class="mord">2</span><span class="msupsub"><span class="vlist-t"><span class="vlist-r"><span class="vlist" style="height: 0.714392em;"><span class="" style="top: -3.113em; margin-right: 0.05em;"><span class="pstrut" style="height: 2.7em;"></span><span class="sizing reset-size6 size3 mtight"><span class="mord mathdefault mtight">m</span></span></span></span></span></span></span></span><span class="mclose">)</span><span class="mspace" style="margin-right: 0.277778em;"></span><span class="mrel">=</span><span class="mspace" style="margin-right: 0.277778em;"></span></span><span class="base"><span class="strut" style="height: 1.188em; vertical-align: -0.25em;"></span><span class="mord">2</span><span class="mord mathdefault" style="margin-right: 0.13889em;">T</span><span class="mopen">(</span><span class="mord"><span class="mord">2</span><span class="msupsub"><span class="vlist-t"><span class="vlist-r"><span class="vlist" style="height: 0.938em;"><span class="" style="top: -3.113em; margin-right: 0.05em;"><span class="pstrut" style="height: 2.7em;"></span><span class="sizing reset-size6 size3 mtight"><span class="mord mtight"><span class="mord mtight">2</span><span class="mord mtight">/</span><span class="mord mathdefault mtight">m</span></span></span></span></span></span></span></span></span><span class="mclose">)</span><span class="mspace" style="margin-right: 0.222222em;"></span><span class="mbin">+</span><span class="mspace" style="margin-right: 0.222222em;"></span></span><span class="base"><span class="strut" style="height: 0.43056em; vertical-align: 0em;"></span><span class="mord mathdefault">m</span></span></span></span></span></span><br>
We can now rename <span class="katex--inline"><span class="katex"><span class="katex-mathml"><math><semantics><mrow><mi>S</mi><mo stretchy="false">(</mo><mi>m</mi><mo stretchy="false">)</mo><mo>=</mo><mi>T</mi><mi>a</mi><mi>m</mi><mi>e</mi><mi>r</mi><mo stretchy="false">(</mo><msup><mn>2</mn><mrow><mn>2</mn><mi mathvariant="normal">/</mi><mi>m</mi></mrow></msup><mo stretchy="false">)</mo></mrow><annotation encoding="application/x-tex">S(m)=Tamer(2^{2/m})</annotation></semantics></math></span><span class="katex-html" aria-hidden="true"><span class="base"><span class="strut" style="height: 1em; vertical-align: -0.25em;"></span><span class="mord mathdefault" style="margin-right: 0.05764em;">S</span><span class="mopen">(</span><span class="mord mathdefault">m</span><span class="mclose">)</span><span class="mspace" style="margin-right: 0.277778em;"></span><span class="mrel">=</span><span class="mspace" style="margin-right: 0.277778em;"></span></span><span class="base"><span class="strut" style="height: 1.138em; vertical-align: -0.25em;"></span><span class="mord mathdefault" style="margin-right: 0.13889em;">T</span><span class="mord mathdefault">a</span><span class="mord mathdefault">m</span><span class="mord mathdefault">e</span><span class="mord mathdefault" style="margin-right: 0.02778em;">r</span><span class="mopen">(</span><span class="mord"><span class="mord">2</span><span class="msupsub"><span class="vlist-t"><span class="vlist-r"><span class="vlist" style="height: 0.888em;"><span class="" style="top: -3.063em; margin-right: 0.05em;"><span class="pstrut" style="height: 2.7em;"></span><span class="sizing reset-size6 size3 mtight"><span class="mord mtight"><span class="mord mtight">2</span><span class="mord mtight">/</span><span class="mord mathdefault mtight">m</span></span></span></span></span></span></span></span></span><span class="mclose">)</span></span></span></span></span> to produce the new recurrence:<br>
<span class="katex--display"><span class="katex-display"><span class="katex"><span class="katex-mathml"><math><semantics><mrow><mi>S</mi><mo stretchy="false">(</mo><mi>m</mi><mo stretchy="false">)</mo><mo>=</mo><mi>S</mi><mo stretchy="false">(</mo><mi>m</mi><mi mathvariant="normal">/</mi><mn>2</mn><mo stretchy="false">)</mo><mo>+</mo><mi>m</mi></mrow><annotation encoding="application/x-tex"> S(m) = S(m/2)+m</annotation></semantics></math></span><span class="katex-html" aria-hidden="true"><span class="base"><span class="strut" style="height: 1em; vertical-align: -0.25em;"></span><span class="mord mathdefault" style="margin-right: 0.05764em;">S</span><span class="mopen">(</span><span class="mord mathdefault">m</span><span class="mclose">)</span><span class="mspace" style="margin-right: 0.277778em;"></span><span class="mrel">=</span><span class="mspace" style="margin-right: 0.277778em;"></span></span><span class="base"><span class="strut" style="height: 1em; vertical-align: -0.25em;"></span><span class="mord mathdefault" style="margin-right: 0.05764em;">S</span><span class="mopen">(</span><span class="mord mathdefault">m</span><span class="mord">/</span><span class="mord">2</span><span class="mclose">)</span><span class="mspace" style="margin-right: 0.222222em;"></span><span class="mbin">+</span><span class="mspace" style="margin-right: 0.222222em;"></span></span><span class="base"><span class="strut" style="height: 0.43056em; vertical-align: 0em;"></span><span class="mord mathdefault">m</span></span></span></span></span></span><br>
which is very much like recurrence (4.19) (<span class="katex--inline"><span class="katex"><span class="katex-mathml"><math><semantics><mrow><mi>T</mi><mo stretchy="false">(</mo><mi>n</mi><mo stretchy="false">)</mo><mo>=</mo><mn>2</mn><mi>T</mi><mo stretchy="false">(</mo><mo stretchy="false">⌈</mo><mi>n</mi><mo stretchy="false">⌉</mo><mo>+</mo><mi>n</mi></mrow><annotation encoding="application/x-tex">T(n) =2T (\lceil n\rceil +n</annotation></semantics></math></span><span class="katex-html" aria-hidden="true"><span class="base"><span class="strut" style="height: 1em; vertical-align: -0.25em;"></span><span class="mord mathdefault" style="margin-right: 0.13889em;">T</span><span class="mopen">(</span><span class="mord mathdefault">n</span><span class="mclose">)</span><span class="mspace" style="margin-right: 0.277778em;"></span><span class="mrel">=</span><span class="mspace" style="margin-right: 0.277778em;"></span></span><span class="base"><span class="strut" style="height: 1em; vertical-align: -0.25em;"></span><span class="mord">2</span><span class="mord mathdefault" style="margin-right: 0.13889em;">T</span><span class="mopen">(</span><span class="mopen">⌈</span><span class="mord mathdefault">n</span><span class="mclose">⌉</span><span class="mspace" style="margin-right: 0.222222em;"></span><span class="mbin">+</span><span class="mspace" style="margin-right: 0.222222em;"></span></span><span class="base"><span class="strut" style="height: 0.43056em; vertical-align: 0em;"></span><span class="mord mathdefault">n</span></span></span></span></span>). Indeed, this new recurrence has the same solution: <span class="katex--inline"><span class="katex"><span class="katex-mathml"><math><semantics><mrow><mi>S</mi><mo stretchy="false">(</mo><mi>m</mi><mo stretchy="false">)</mo><mo>=</mo><mi>O</mi><mo stretchy="false">(</mo><mi>m</mi><mo>∗</mo><mi>l</mi><mi>g</mi><mo stretchy="false">(</mo><mi>m</mi><mo stretchy="false">)</mo><mo stretchy="false">)</mo></mrow><annotation encoding="application/x-tex">S(m)=O(m*lg(m))</annotation></semantics></math></span><span class="katex-html" aria-hidden="true"><span class="base"><span class="strut" style="height: 1em; vertical-align: -0.25em;"></span><span class="mord mathdefault" style="margin-right: 0.05764em;">S</span><span class="mopen">(</span><span class="mord mathdefault">m</span><span class="mclose">)</span><span class="mspace" style="margin-right: 0.277778em;"></span><span class="mrel">=</span><span class="mspace" style="margin-right: 0.277778em;"></span></span><span class="base"><span class="strut" style="height: 1em; vertical-align: -0.25em;"></span><span class="mord mathdefault" style="margin-right: 0.02778em;">O</span><span class="mopen">(</span><span class="mord mathdefault">m</span><span class="mspace" style="margin-right: 0.222222em;"></span><span class="mbin">∗</span><span class="mspace" style="margin-right: 0.222222em;"></span></span><span class="base"><span class="strut" style="height: 1em; vertical-align: -0.25em;"></span><span class="mord mathdefault" style="margin-right: 0.01968em;">l</span><span class="mord mathdefault" style="margin-right: 0.03588em;">g</span><span class="mopen">(</span><span class="mord mathdefault">m</span><span class="mclose">)</span><span class="mclose">)</span></span></span></span></span> Changing back from <span class="katex--inline"><span class="katex"><span class="katex-mathml"><math><semantics><mrow><mi>S</mi><mo stretchy="false">(</mo><mi>m</mi><mo stretchy="false">)</mo><mi>t</mi><mi>o</mi><mi>T</mi><mo stretchy="false">(</mo><mi>n</mi><mo stretchy="false">)</mo></mrow><annotation encoding="application/x-tex">S(m) to T(n)</annotation></semantics></math></span><span class="katex-html" aria-hidden="true"><span class="base"><span class="strut" style="height: 1em; vertical-align: -0.25em;"></span><span class="mord mathdefault" style="margin-right: 0.05764em;">S</span><span class="mopen">(</span><span class="mord mathdefault">m</span><span class="mclose">)</span><span class="mord mathdefault">t</span><span class="mord mathdefault">o</span><span class="mord mathdefault" style="margin-right: 0.13889em;">T</span><span class="mopen">(</span><span class="mord mathdefault">n</span><span class="mclose">)</span></span></span></span></span> we obtain<br>
<span class="katex--inline"><span class="katex"><span class="katex-mathml"><math><semantics><mrow><mi>T</mi><mo stretchy="false">(</mo><mi>n</mi><mo stretchy="false">)</mo><mo>=</mo><msup><mi>T</mi><mrow><mn>2</mn><mi>m</mi></mrow></msup><mo>=</mo><mi>S</mi><mo stretchy="false">(</mo><mi>m</mi><mo stretchy="false">)</mo><mo>=</mo><mi>O</mi><mo stretchy="false">(</mo><mi>m</mi><mo>∗</mo><mi>l</mi><mi>g</mi><mo stretchy="false">(</mo><mi>m</mi><mo stretchy="false">)</mo><mo>=</mo><mi>O</mi><mo stretchy="false">(</mo><mi>l</mi><mi>g</mi><mo stretchy="false">(</mo><mi>n</mi><mo stretchy="false">)</mo><mi>l</mi><mi>g</mi><mo stretchy="false">(</mo><mi>l</mi><mi>g</mi><mo stretchy="false">(</mo><mi>n</mi><mo stretchy="false">)</mo><mo stretchy="false">)</mo></mrow><annotation encoding="application/x-tex">T(n)=T^{2m} = S(m)= O(m*lg(m) = O(lg (n )lg( lg (n))</annotation></semantics></math></span><span class="katex-html" aria-hidden="true"><span class="base"><span class="strut" style="height: 1em; vertical-align: -0.25em;"></span><span class="mord mathdefault" style="margin-right: 0.13889em;">T</span><span class="mopen">(</span><span class="mord mathdefault">n</span><span class="mclose">)</span><span class="mspace" style="margin-right: 0.277778em;"></span><span class="mrel">=</span><span class="mspace" style="margin-right: 0.277778em;"></span></span><span class="base"><span class="strut" style="height: 0.814108em; vertical-align: 0em;"></span><span class="mord"><span class="mord mathdefault" style="margin-right: 0.13889em;">T</span><span class="msupsub"><span class="vlist-t"><span class="vlist-r"><span class="vlist" style="height: 0.814108em;"><span class="" style="top: -3.063em; margin-right: 0.05em;"><span class="pstrut" style="height: 2.7em;"></span><span class="sizing reset-size6 size3 mtight"><span class="mord mtight"><span class="mord mtight">2</span><span class="mord mathdefault mtight">m</span></span></span></span></span></span></span></span></span><span class="mspace" style="margin-right: 0.277778em;"></span><span class="mrel">=</span><span class="mspace" style="margin-right: 0.277778em;"></span></span><span class="base"><span class="strut" style="height: 1em; vertical-align: -0.25em;"></span><span class="mord mathdefault" style="margin-right: 0.05764em;">S</span><span class="mopen">(</span><span class="mord mathdefault">m</span><span class="mclose">)</span><span class="mspace" style="margin-right: 0.277778em;"></span><span class="mrel">=</span><span class="mspace" style="margin-right: 0.277778em;"></span></span><span class="base"><span class="strut" style="height: 1em; vertical-align: -0.25em;"></span><span class="mord mathdefault" style="margin-right: 0.02778em;">O</span><span class="mopen">(</span><span class="mord mathdefault">m</span><span class="mspace" style="margin-right: 0.222222em;"></span><span class="mbin">∗</span><span class="mspace" style="margin-right: 0.222222em;"></span></span><span class="base"><span class="strut" style="height: 1em; vertical-align: -0.25em;"></span><span class="mord mathdefault" style="margin-right: 0.01968em;">l</span><span class="mord mathdefault" style="margin-right: 0.03588em;">g</span><span class="mopen">(</span><span class="mord mathdefault">m</span><span class="mclose">)</span><span class="mspace" style="margin-right: 0.277778em;"></span><span class="mrel">=</span><span class="mspace" style="margin-right: 0.277778em;"></span></span><span class="base"><span class="strut" style="height: 1em; vertical-align: -0.25em;"></span><span class="mord mathdefault" style="margin-right: 0.02778em;">O</span><span class="mopen">(</span><span class="mord mathdefault" style="margin-right: 0.01968em;">l</span><span class="mord mathdefault" style="margin-right: 0.03588em;">g</span><span class="mopen">(</span><span class="mord mathdefault">n</span><span class="mclose">)</span><span class="mord mathdefault" style="margin-right: 0.01968em;">l</span><span class="mord mathdefault" style="margin-right: 0.03588em;">g</span><span class="mopen">(</span><span class="mord mathdefault" style="margin-right: 0.01968em;">l</span><span class="mord mathdefault" style="margin-right: 0.03588em;">g</span><span class="mopen">(</span><span class="mord mathdefault">n</span><span class="mclose">)</span><span class="mclose">)</span></span></span></span></span></p>
<h2 id="the-akra-bazzi-method-if-possible-since-its-hard-af">The Akra-Bazzi method (if possible since it’s HARD af)</h2>
<p>P-113</p>
<h2 id="go-back-to-growth-functions">Go back to Growth Functions</h2>
<p>Problems : P62-63</p>
<h2 id="plz-do-some-algorithms-solving-problems-recursion-recurrence-functions">Plz do some algorithms (solving problems, recursion, recurrence functions)</h2>
<p>Problems : P39-42 , P107-111</p>

